update to coq bank account example & soundness proof

coq_inference/bank_account.v
@@ -44,6 +44,8 @@ Module BankAccount(L : LanguageDef).
 
   Definition pwd := (n_ 101).
 
+  Definition newPwd := (n_ 205).
+
   (** #<h2>#Ledger Class#</h2># *)
 
   Definition Ledger := classID 200.
@@ -115,34 +117,40 @@ Module BankAccount(L : LanguageDef).
   (** #<h2>#Account Specifications#</h2># *)
 
   Parameter authenticateBalanceChangeSpecification :
-    forall a a' b β bal, BankMdl ⊢ {pre: (a_class (e_ a) Account) ∧
-                                    (a_class (e_ a') Account) ∧
+    forall a a' b β bal, BankMdl ⊢ {pre: (a_class (e_ a') Account) ∧
                                     (a_class (e_ b)  Bank) ∧
-                                    (a_exp ((e_acc_g (e_ b) getBalance (e_ a')) ⩵ (e_int bal)))}
+                                    (a_exp ((e_acc_g (e_ b) getBalance (e_ a')) ⩵ (e_int bal))) ∧
+                                    (a_class (e_ a) Account)}
                             m_call a authenticate β
                             {post: a_exp ((e_acc_g (e_ b) getBalance (e_ a')) ⩵ (e_int bal))}.
 
   Parameter changePasswordBalanceChangeSpecification :
-    forall a a' b β bal, BankMdl ⊢ {pre: (a_class (e_ a) Account) ∧
-                                    (a_class (e_ a') Account) ∧
+    forall a a' b β bal, BankMdl ⊢ {pre: (a_class (e_ a') Account) ∧
                                     (a_class (e_ b)  Bank) ∧
-                                    (a_exp ((e_acc_g (e_ b) getBalance (e_ a')) ⩵ (e_int bal)))}
+                                    (a_exp ((e_acc_g (e_ b) getBalance (e_ a')) ⩵ (e_int bal))) ∧
+                                    (a_class (e_ a) Account)}
                             m_call a changePassword β
                             {post: a_exp ((e_acc_g (e_ b) getBalance (e_ a')) ⩵ (e_int bal))}.
 
   Parameter transferBalanceChangeSpecification :
-    forall a a' b b' p bal β,
+    forall a a' b b' p p' bal β,
       BankMdl ⊢ {pre: (a_class (e_ a) Account) ∧
                       (a_class (e_ b)  Bank) ∧
+                      (a_exp ((e_acc_g (e_ b) getBalance (e_ a)) ⩵ (e_int bal))) ∧
+                      (a_exp ((e_acc_f (e_ a) password) ⩵ (e_val p))) ∧
                       (a_class (e_ b') Bank) ∧
-                      (a_exp ((e_acc_g (e_ b) getBalance (e_ a)) ⩵ (e_int bal)))}
-              m_call b' transfer (⟦ pwd ↦ p⟧ ⟦ fromAcc ↦ a' ⟧ β)
-              {post: a_exp (e_val p ⩵ e_acc_f (e_ a) password) ∧
-                     (a_exp (e_val a' ⩵ (e_ a))) ∧
-                     (a_exp (e_ b' ⩵ (e_ b)))}.
+                      (¬ ((a_exp (e_val p' ⩵ e_val p)) ∧
+                          (a_exp (e_val a' ⩵ e_ a)) ∧
+                          (a_exp (e_ b' ⩵ e_ b))))}
+              m_call b' transfer (⟦ pwd ↦ p'⟧ ⟦ fromAcc ↦ a' ⟧ β)
+              {post: (¬ a_exp (e_acc_g (e_ b) getBalance (e_ a) ⩻ (e_int bal)))}.
 
   Lemma eq_implies_not_lt :
     forall M e1 e2, M ⊢ (a_exp (e1 ⩵ e2)) ⊇ (¬ a_exp (e1 ⩻ e2)).
+  Admitted.
+
+  Lemma lt_implies_not_eq :
+    forall M e1 e2, M ⊢ (a_exp (e1 ⩻ e2)) ⊇ (¬ a_exp (e1 ⩵ e2)).
   Admitted.
 
   Lemma not_false_is_true :
@@ -193,6 +201,12 @@ Module BankAccount(L : LanguageDef).
                    M ⊢ A1 ∧ A2 ⊇ A2'.
   Admitted.
 
+  Lemma conseq_and :
+    forall M A A1 A2,  M ⊢ A ⊇ A1 ->
+                  M ⊢ A ⊇ A2 ->
+                  M ⊢ A ⊇ A1 ∧ A2.
+  Admitted.
+
   Lemma conseq_ex :
     forall M A1 A2, (forall x, M ⊢ [x /s 0] A1 ⊇ A2) ->
                M ⊢ (∃x.[A1]) ⊇ A2.
@@ -215,6 +229,24 @@ Module BankAccount(L : LanguageDef).
   Lemma param_unique :
     forall M a1 a1' a2 a2' m m' x v v' β β',
       M ⊢ a1 calls a2 ◌ m ⟨ ⟦ x ↦ (av_ v) ⟧ β ⟩ ∧ a1' calls a2' ◌ m' ⟨ ⟦ x ↦ (av_ v') ⟧ β' ⟩ ⊇ (a_exp ((e_val v) ⩵ (e_val v'))).
+  Admitted.
+
+  Lemma neg_distr_and_1 :
+    forall M A1 A2, M ⊢ ¬ (A1 ∧ A2) ⊇ ¬ A1 ∨ ¬ A2.
+  Admitted.
+
+  Lemma neg_distr_and_2 :
+    forall M A1 A2, M ⊢ ¬ A1 ∨ ¬ A2 ⊇ ¬ (A1 ∧ A2).
+  Admitted.
+
+  Lemma or_l :
+    forall M A A1 A2, M ⊢ A ⊇ A1 ->
+                 M ⊢ A ⊇ A1 ∨ A2.
+  Admitted.
+
+  Lemma or_r :
+    forall M A A1 A2, M ⊢ A ⊇ A2 ->
+                 M ⊢ A ⊇ A1 ∨ A2.
   Admitted.
 
   Ltac hoare_simpl :=
@@ -250,6 +282,8 @@ Module BankAccount(L : LanguageDef).
      apply conseq_and2, conseq_and1
     |[|- _ ⊢ _ ∧ _ ∧ ?A ∧ _ ⊇ ?A] =>
      apply conseq_and2, conseq_and2, conseq_and1
+    |[|- _ ⊢ _ ⊇ _ ∧ _] =>
+     apply conseq_and
     end.
 
   Lemma authBalChange :
@@ -295,19 +329,19 @@ Module BankAccount(L : LanguageDef).
                  (a_class (e_ b) Bank) ∧
                  (a_exp ((e_acc_g (e_ b) getBalance (e_ a)) ⩵ (e_int bal))) ∧
                  (a_exp ((e_acc_f (e_ a) password) ⩵ (e_val v))) ∧
-                (∃x.[ (a♢ 0) calls (a_ l) ◌ ledgerTransfer ⟨ ps ⟩ ]))
+                 (∃x.[ (a♢ 0) calls (a_ l) ◌ ledgerTransfer ⟨ ps ⟩ ]))
               to1 (a_exp ((e_acc_g (e_ b) getBalance (e_ a)) ⩻ (e_int bal)))
               onlyIf (∃x.[∃x.[∃x.[ (a♢ 0) calls (a_ b) ◌ transfer ⟨ ⟦ pwd ↦ (av_ v)⟧
-                                                                                ⟦ amt ↦ (a♢ 1)⟧
-                                                                                ⟦ fromAcc ↦ (a_ a) ⟧
-                                                                                ⟦ toAcc ↦ (a♢ 2) ⟧
-                                                                                empty ⟩]]]).
+                                                                      ⟦ fromAcc ↦ (a_ a) ⟧
+                                                                      ⟦ amt ↦ (a♢ 1)⟧
+                                                                      ⟦ toAcc ↦ (a♢ 2) ⟧
+                                                                      empty ⟩]]]).
   Proof.
     intros.
     eapply (if1_conseq);
       [|apply conseq_refl
        |apply conseq_refl
-       |apply absurd].
+       |apply conseq_absurd].
     eapply (if1_conseq);
       [|apply conseq_refl
        |apply conseq_refl
@@ -315,64 +349,388 @@ Module BankAccount(L : LanguageDef).
     apply if1_andI.
 
     - apply if1_if.
-      apply if_start.
+      eapply if_conseq;
+        [ apply if_start
+        | apply conseq_refl
+        | apply conseq_refl
+        | ].
       apply consequence_transitivity with (A2 := a_class (e_ l) Ledger);
         [apply conseq_and1|apply inside_wrapped with (Def:=LedgerDef); auto].
       repeat apply conseq_and1; spec_auto.
 
-    - apply if1_if, if_start.
+    - eapply if1_if, if_conseq;
+        [ apply if_start
+        | apply conseq_refl
+        | apply conseq_refl
+        | ].
       repeat apply conseq_and2.
       spec_auto.
       apply recv_not_wrapped.
   Qed.
 
-  Lemma bankTransferBalChange :
-    forall a b b' bal p p' ps,
+  Lemma if1_start :
+    forall M A1 A2, M ⊢ A1 to1 A2 onlyIf A1.
+  Proof.
+    auto with inference_db.
+  Qed.
+
+  Hint Resolve if1_start : inference_db.
+
+  Lemma if1_conseq1 :
+    forall M A1 A2 A3 A1', M ⊢ A1' ⊇ A1 ->
+                      M ⊢ A1 to1 A2 onlyIf A3 ->
+                      M ⊢ A1' to1 A2 onlyIf A3.
+  Proof.
+    intros.
+    eapply if1_conseq;
+      try solve [eauto];
+      try solve [apply conseq_refl].
+  Qed.
+
+  Lemma if1_conseq2 :
+    forall M A1 A2 A3 A2', M ⊢ A2' ⊇ A2 ->
+                      M ⊢ A1 to1 A2 onlyIf A3 ->
+                      M ⊢ A1 to1 A2' onlyIf A3.
+  Proof.
+    intros.
+    eapply if1_conseq;
+      try solve [eauto];
+      try solve [apply conseq_refl].
+  Qed.
+
+  Lemma if1_conseq3 :
+    forall M A1 A2 A3 A3', M ⊢ A3 ⊇ A3' ->
+                      M ⊢ A1 to1 A2 onlyIf A3 ->
+                      M ⊢ A1 to1 A2 onlyIf A3'.
+  Proof.
+    intros.
+    eapply if1_conseq;
+      try solve [eauto];
+      try solve [apply conseq_refl].
+  Qed.
+
+  Hint Resolve if1_conseq1 if1_conseq2 if1_conseq3 : inference_db.
+
+  Lemma if_conseq1 :
+    forall M A1 A2 A3 A1', M ⊢ A1' ⊇ A1 ->
+                      M ⊢ A1 to A2 onlyIf A3 ->
+                      M ⊢ A1' to A2 onlyIf A3.
+  Proof.
+    intros.
+    eapply if_conseq;
+      try solve [eauto];
+      try solve [apply conseq_refl].
+  Qed.
+
+  Lemma if_conseq2 :
+    forall M A1 A2 A3 A2', M ⊢ A2' ⊇ A2 ->
+                      M ⊢ A1 to A2 onlyIf A3 ->
+                      M ⊢ A1 to A2' onlyIf A3.
+  Proof.
+    intros.
+    eapply if_conseq;
+      try solve [eauto];
+      try solve [apply conseq_refl].
+  Qed.
+
+  Lemma if_conseq3 :
+    forall M A1 A2 A3 A3', M ⊢ A3 ⊇ A3' ->
+                      M ⊢ A1 to A2 onlyIf A3 ->
+                      M ⊢ A1 to A2 onlyIf A3'.
+  Proof.
+    intros.
+    eapply if_conseq;
+      try solve [eauto];
+      try solve [apply conseq_refl].
+  Qed.
+
+  Hint Resolve if_conseq1 if_conseq2 if_conseq3 : inference_db.
+
+  Lemma ot_conseq1 :
+    forall M A1 A2 A3 A1', M ⊢ A1' ⊇ A1 ->
+                      M ⊢ A1 to A2 onlyThrough A3 ->
+                      M ⊢ A1' to A2 onlyThrough A3.
+  Proof.
+    intros.
+    eapply ot_conseq;
+      try solve [eauto];
+      try solve [apply conseq_refl].
+  Qed.
+
+  Lemma ot_conseq2 :
+    forall M A1 A2 A3 A2', M ⊢ A2' ⊇ A2 ->
+                      M ⊢ A1 to A2 onlyThrough A3 ->
+                      M ⊢ A1 to A2' onlyThrough A3.
+  Proof.
+    intros.
+    eapply ot_conseq;
+      try solve [eauto];
+      try solve [apply conseq_refl].
+  Qed.
+
+  Lemma ot_conseq3 :
+    forall M A1 A2 A3 A3', M ⊢ A3 ⊇ A3' ->
+                      M ⊢ A1 to A2 onlyThrough A3 ->
+                      M ⊢ A1 to A2 onlyThrough A3'.
+  Proof.
+    intros.
+    eapply ot_conseq;
+      try solve [eauto];
+      try solve [apply conseq_refl].
+  Qed.
+
+  Hint Resolve ot_conseq1 ot_conseq2 ot_conseq3 : inference_db.
+
+  Lemma if1_start_conseq :
+    forall M A1 A2 A1', M ⊢ A1 ⊇ A1' ->
+                   M ⊢ A1 to1 A2 onlyIf A1'.
+  Proof.
+    intros.
+    eapply if1_conseq3;
+      eauto with inference_db.
+  Qed.
+
+  Hint Resolve if1_start if1_start_conseq : inference_db.
+
+  Lemma if_start_conseq :
+    forall M A1 A2 A1', M ⊢ A1 ⊇ A1' ->
+                   M ⊢ A1 to A2 onlyIf A1'.
+  Proof.
+    intros.
+    eapply if_conseq3;
+      eauto with inference_db.
+  Qed.
+
+  Hint Resolve if_start_conseq : inference_db.
+
+  Lemma if1_andE :
+    forall M A1 A2 A A', M ⊢ A1 to1 A2 onlyIf A ∧ A' ->
+                    M ⊢ A1 to1 A2 onlyIf A.
+  Proof.
+    intros.
+    eapply if1_conseq with (A':=A ∧ A');
+      [ eauto
+      | apply conseq_refl
+      | apply conseq_refl
+      | apply conseq_and1, conseq_refl].
+  Qed.
+
+  Lemma compose_update :
+    forall {A B C : Type}`{Eq A} (f : B -> C) (a : A) (b : B) (g : partial_map A B),
+      (fun b => Some (f b)) ∘ (⟦ a ↦ b ⟧ g) = ⟦ a ↦ f b ⟧ (fun b => Some (f b)) ∘ g.
+  Proof.
+    intros.
+    simpl.
+    apply functional_extensionality;
+      intros.
+    repeat map_rewrite.
+    destruct (eqb x a);
+      auto.
+  Qed.
+
+  Lemma compose_empty :
+    forall {A B C}`{Eq A} (f : B -> C),
+      (fun b => Some (f b)) ∘ empty = empty.
+  Proof.
+    intros;
+      auto.
+  Qed.
+
+  Ltac compose_simpl :=
+    match goal with
+    | [|- context[(fun _ => Some (?f _)) ∘ ⟦ _ ↦ _ ⟧ _]] =>
+      rewrite compose_update
+    | [H : context[(fun _ => Some (?f _)) ∘ ⟦ _ ↦ _ ⟧ _] |- _] =>
+      rewrite compose_update in H
+    | [|- context[(fun _ => Some (?f _)) ∘ empty]] =>
+      rewrite compose_empty
+    | [H : context[(fun _ => Some (?f _)) ∘ empty] |- _] =>
+      rewrite compose_empty in H
+    end.
+
+  Lemma bankTransferBalChange' :
+    forall a b b' bal p p' a' m a'',
       BankMdl ⊢ ((a_class (e_ a) Account) ∧
                  (a_class (e_ b) Bank) ∧
-                 (a_class (e_ b') Bank) ∧
                  (a_exp ((e_acc_g (e_ b) getBalance (e_ a)) ⩵ (e_int bal))) ∧
                  (a_exp ((e_acc_f (e_ a) password) ⩵ (e_ p))) ∧
-                (∃x.[ (a♢ 0) calls (a_ b') ◌ transfer ⟨ ⟦ pwd ↦ a_ p' ⟧ ps  ⟩ ]))
+                 (a_class (e_ b') Bank) ∧
+                 (∃x.[ (a♢ 0) calls (a_ b') ◌ transfer ⟨ ⟦ pwd ↦ a_ p' ⟧
+                                                           ⟦ fromAcc ↦ a_ a' ⟧
+                                                           ⟦ amt ↦ av_ m ⟧
+                                                           ⟦ toAcc ↦ av_ a'' ⟧
+                                                           empty  ⟩ ]))
               to1 (a_exp ((e_acc_g (e_ b) getBalance (e_ a)) ⩻ (e_int bal)))
-              onlyIf (∃x.[∃x.[∃x.[ (a♢ 0) calls (a♢ 1) ◌ transfer ⟨ ⟦ pwd ↦ (a_ p)⟧
-                                                                      ⟦ amt ↦ (a♢ 2)⟧
-                                                                      ⟦ fromAcc ↦ (a♢ 3) ⟧
-                                                                      ⟦ toAcc ↦ (a♢ 4) ⟧
-                                                                      empty ⟩]]]).
+              onlyIf (a_exp (e_ p' ⩵ e_ p) ∧ (a_exp (e_ a' ⩵ e_ a)) ∧ (a_exp (e_ b' ⩵ e_ b))).
   Proof.
     intros.
 
-    extract3 (v_ p) 100;
+    apply if1_classical with (β:=⟦ pwd ↦ v_ p' ⟧
+                                   ⟦ fromAcc ↦ v_ a' ⟧
+                                   ⟦ amt ↦ m ⟧
+                                   ⟦ toAcc ↦ a'' ⟧
+                                   empty);
+      [|repeat compose_simpl; auto].
+    repeat hoare_simpl.
+
+    apply transferBalanceChangeSpecification.
+
+(*    apply hoare_consequence1 with
+        (A1':=(a_class (e_addr a) Account) ∧
+              (a_class (e_addr b) Bank) ∧
+              (a_exp (e_acc_g (e_addr b) getBalance (e_addr a) ⩵ (e_int bal))) ∧
+              (a_exp (e_acc_f (e_addr a) password ⩵ (e_addr p))) ∧
+              (a_class (e_addr b') Bank) ∧
+              ¬ (a_exp (e_ p' ⩵ e_ p) ∧
+                 a_exp (e_ a' ⩵ e_ a) ∧
+                 a_exp (e_ b' ⩵ e_ b))).
+
+      - apply transferBalanceChangeSpecification.
+
+    - repeat spec_auto.
+      apply conseq_and2.
+      match goal with
+      | [|- _ ⊢ _ ⊇ ¬ (?Aa ∧ ?Ab)] =>
+        apply consequence_transitivity with (A2:= ¬ Aa ∨ ¬ Ab)
+      end.
+      + apply or_l, conseq_refl.
+
+      + apply neg_distr_and_2.*)
+
+  Qed.
+
+  Lemma bankTransferBalChange :
+    forall a b b' bal p p' a' m a'',
+      BankMdl ⊢ ((a_class (e_ a) Account) ∧
+                 (a_class (e_ b) Bank) ∧
+                 (a_exp ((e_acc_g (e_ b) getBalance (e_ a)) ⩵ (e_int bal))) ∧
+                 (a_exp ((e_acc_f (e_ a) password) ⩵ (e_ p))) ∧
+                 (a_class (e_ b') Bank) ∧
+                 (∃x.[ (a♢ 0) calls (a_ b') ◌ transfer ⟨ ⟦ pwd ↦ a_ p' ⟧
+                                                           ⟦ fromAcc ↦ a_ a' ⟧
+                                                           ⟦ amt ↦ av_ m ⟧
+                                                           ⟦ toAcc ↦ av_ a'' ⟧
+                                                           empty  ⟩ ]))
+              to1 (a_exp ((e_acc_g (e_ b) getBalance (e_ a)) ⩻ (e_int bal)))
+              onlyIf (∃x.[ ∃x.[ ∃x.[ (a♢ 0) calls (a_ b) ◌ transfer ⟨ ⟦ pwd ↦ a_ p ⟧
+                                                                        ⟦ fromAcc ↦ a_ a ⟧
+                                                                        ⟦ amt ↦ a♢ 1 ⟧
+                                                                        ⟦ toAcc ↦ a♢ 2 ⟧
+                                                                        empty  ⟩ ]]]).
+  Proof.
+    intros.
+    match goal with
+    | [|- _ ⊢  _ to1 _ onlyIf _] =>
       eapply if1_conseq;
-      [|apply conseq_refl
-       |apply conseq_refl
-       |apply subst_eq with (y:=v_ p'); simpl];
-      subst_simpl.
+        [apply if1_start
+        |apply conseq_refl
+        |apply conseq_refl
+        |]
+    end.
+    repeat spec_auto.
+  Admitted.
 
-    eapply if1_andI.
-
-    - eapply if1_if.
-      eapply if_start.
-      eapply conseq_and1, conseq_and2.
-      
-
-
-    extract3 (v_ a) 100;
-      eapply if1_conseq;
-      [|apply conseq_refl
-       |apply conseq_refl
-       |apply subst_eq with (y:=v_ b); simpl];
-      subst_simpl.
-
-    eapply if1_classical;
-      [|auto].
+  Lemma balanceChange :
+    forall a b bal p,
+      BankMdl ⊢ ((a_class (e_ a) Account) ∧
+                 (a_class (e_ b) Bank) ∧
+                 (a_exp ((e_acc_g (e_ b) getBalance (e_ a)) ⩵ (e_int bal))) ∧
+                 (a_exp ((e_acc_f (e_ a) password) ⩵ (e_ p))))
+              to1 (a_exp ((e_acc_g (e_ b) getBalance (e_ a)) ⩻ (e_int bal)))
+              onlyIf (∃x.[ ∃x.[ ∃x.[ (a♢ 0) calls (a_ b) ◌ transfer ⟨ ⟦ pwd ↦ a_ p ⟧
+                                                                        ⟦ fromAcc ↦ a_ a ⟧
+                                                                        ⟦ toAcc ↦ a♢ 1 ⟧
+                                                                        ⟦ amt ↦ a♢ 2 ⟧
+                                                                        empty  ⟩ ]]]).
+  Proof.
 
   Admitted.
 
-  Lemma balanceEncaps :
-    forall b b' a bal 
+  Lemma balanceChange' :
+    forall a b bal p,
+      BankMdl ⊢ ((a_class (e_ a) Account) ∧
+                 (a_class (e_ b) Bank) ∧
+                 (a_exp ((e_acc_g (e_ b) getBalance (e_ a)) ⩵ (e_int bal))) ∧
+                 (a_exp ((e_acc_f (e_ a) password) ⩵ (e_ p))))
+              to (a_exp ((e_acc_g (e_ b) getBalance (e_ a)) ⩻ (e_int bal)))
+              onlyThrough ∃x.[ ¬ wrapped (a♢ 0) ∧
+                               (a_exp (e_acc_f (e_ a) password ⩵ (e♢ 0)))].
+  Proof.
 
+  Admitted.
+
+  Lemma passwordChange :
+    forall a p, BankMdl ⊢ (a_class (e_ a) Account ∧
+                      (a_exp (e_acc_f (e_ a) password ⩵ e_ p)))
+                   to1 (¬ a_exp (e_acc_f (e_ a) password ⩵ e_ p))
+                   onlyIf (∃x.[ ∃x.[ (a♢ 0) calls (a_ a) ◌ changePassword ⟨ ⟦ pwd ↦ a_ p ⟧ ⟦ newPwd ↦ a♢ 1 ⟧ empty  ⟩ ] ]).
+  Proof.
+
+  Admitted.
+
+  Lemma passwordLeak :
+    forall a p, BankMdl ⊢ (a_class (e_ a) Account ∧
+                      (a_exp (e_acc_f (e_ a) password ⩵ e_ p) ∧
+                       (wrapped (a_ p))))
+                   to (¬ (wrapped (a_ p)))
+                   onlyIf (a_exp (e_false)).
+  Proof.
+
+  Admitted.
+
+  Lemma or_dumb1 :
+    forall M A, M ⊢ A ⊇ A ∨ A.
+  Proof.
+  Admitted.
+
+  Lemma or_dumb2 :
+    forall M A, M ⊢ A ∨ A ⊇ A.
+  Proof.
+  Admitted.
+
+  Lemma conseq_excluded_middle :
+    forall M A, M ⊢ (a_exp (e_true)) ⊇ (A ∨ ¬ A).
+  Admitted.
+
+  Lemma necessityBankSpec :
+    forall a b bal p, BankMdl ⊢ (a_class (e_ a) Account ∧
+                            a_class (e_ b) Bank ∧
+                            (a_exp (e_acc_g (e_ b) getBalance (e_ a) ⩵ (e_int bal))) ∧
+                            (a_exp (e_acc_f (e_ a) password ⩵ (e_ p))))
+                         to (a_exp (e_acc_g (e_ b) getBalance (e_ a) ⩻ (e_int bal)))
+                         onlyIf ¬ wrapped (a_ p).
+  Proof.
+    intros.
+    apply if_trans with (A':= ¬ wrapped (a_ p) ∨ ¬ (a_exp (e_acc_f (e_ a) password ⩵ (e_ p)))).
+
+    - apply ot_conseq3 with (A3:=∃x.[ ¬ wrapped (a♢ 0) ∧
+                                      (a_exp (e_acc_f (e_ a) password ⩵ (e♢ 0)))]).
+      + admit. (* basic from natural deduction. need to encode *)
+
+      + apply balanceChange'.
+
+    - apply if_conseq3 with (A3:= ¬ wrapped (a_ p) ∨ ¬ wrapped (a_ p));
+        [apply or_dumb2|].
+      apply if_orI2.
+
+      * (* Case A *)
+        apply if_orE with (A':= wrapped (a_ p)).
+
+      + admit. (* excluded middle*)
+      + apply ot_conseq1 with (A1:=a_class (e_ a) Account ∧
+                                   (a_exp (e_acc_f (e_ a) password ⩵ (e_ p)) ∧
+                                   wrapped (a_ p))).
+        ++ repeat spec_auto.
+           +++ admit. (* easy *)
+           +++ admit. (* easy *)
+
+        ++ apply ot_if.
+           apply passwordLeak.
+
+
+      * (* Case B *)
+        
+  Qed.
 
   Close Scope chainmail_scope.
   Close Scope reduce_scope.
